Seperate expession typing and use mutual induction

Typing.thy
@@ -5,8 +5,7 @@ begin
 no_notation Set.member  ("(_/ : _)" [51, 51] 50)
 
 inductive Ctx :: "\<Gamma> \<Rightarrow> bool" ("\<turnstile> _")
-  and Ty :: "\<Gamma> \<Rightarrow> \<tau> \<Rightarrow> \<kappa> \<Rightarrow> bool" ("_ \<turnstile>\<^sub>t\<^sub>y _ : _")
-  and Tm :: "\<Gamma> \<Rightarrow> term \<Rightarrow> \<tau> \<Rightarrow> bool" ("_ \<turnstile> _ : _" 50) where
+  and Ty :: "\<Gamma> \<Rightarrow> \<tau> \<Rightarrow> \<kappa> \<Rightarrow> bool" ("_ \<turnstile>\<^sub>t\<^sub>y _ : _") where
 
   Ctx_Empty: "\<turnstile> []"
 
@@ -26,9 +25,10 @@ inductive Ctx :: "\<Gamma> \<Rightarrow> bool" ("\<turnstile> _")
 
 | Ty_Forall: "\<lbrakk> BTyVar a k # \<Gamma> \<turnstile>\<^sub>t\<^sub>y \<sigma> : \<star> \<rbrakk> \<Longrightarrow> \<Gamma> \<turnstile>\<^sub>t\<^sub>y (\<forall>a : k. \<sigma>) : \<star>"
 
-(* ------------------------------ *)
+equivariance Ctx
 
-| Tm_Var: "\<lbrakk> \<turnstile> \<Gamma> ; BVar x \<tau> \<in> \<Gamma> \<rbrakk> \<Longrightarrow> \<Gamma> \<turnstile> (Var x) : \<tau>"
+inductive Tm :: "\<Gamma> \<Rightarrow> term \<Rightarrow> \<tau> \<Rightarrow> bool" ("_ \<turnstile> _ : _" 50) where
+  Tm_Var: "\<lbrakk> \<turnstile> \<Gamma> ; BVar x \<tau> \<in> \<Gamma> \<rbrakk> \<Longrightarrow> \<Gamma> \<turnstile> (Var x) : \<tau>"
 
 | Tm_Abs: "BVar x \<tau>1 # \<Gamma> \<turnstile> e : \<tau>2 \<Longrightarrow> \<Gamma> \<turnstile> (\<lambda> x : \<tau>1 . e) : (\<tau>1 \<rightarrow> \<tau>2)"
 
@@ -42,11 +42,10 @@ inductive Ctx :: "\<Gamma> \<Rightarrow> bool" ("\<turnstile> _")
 
 | Tm_Let: "\<lbrakk> \<Gamma> \<turnstile> e1 : \<tau>1 ; BVar x \<tau>1 # \<Gamma> \<turnstile> e2 : \<tau>2 \<rbrakk> \<Longrightarrow> \<Gamma> \<turnstile> Let x \<tau>1 e1 e2 : \<tau>2"
 
-equivariance Ctx
+equivariance Tm
 
-lemmas Ctx_intros = Ctx_Ty_Tm.intros(1-3)
-lemmas Ty_intros = Ctx_Ty_Tm.intros(4-8)
-lemmas Tm_intros = Ctx_Ty_Tm.intros(9-15)
+lemmas Ctx_intros = Ctx_Ty.intros(1-3)
+lemmas Ty_intros = Ctx_Ty.intros(4-8)
 
 inductive_cases CtxE[elim]:
   "\<turnstile> BTyVar a k # \<Gamma>"
@@ -71,7 +70,7 @@ lemma Ctx_induct[consumes 1, case_names Empty TyVar Var]:
   and TyVar: "\<And>\<Gamma> a k. \<lbrakk> \<turnstile> \<Gamma> ; P \<Gamma> ; atom a \<sharp> \<Gamma> \<rbrakk> \<Longrightarrow> P (BTyVar a k # \<Gamma>)"
   and Var: "\<And>\<Gamma> x \<tau>. \<lbrakk> \<Gamma> \<turnstile>\<^sub>t\<^sub>y \<tau> : \<star> ; atom x \<sharp> \<Gamma> \<rbrakk> \<Longrightarrow> P (BVar x \<tau> # \<Gamma>)"
 shows "P \<Gamma>"
-  using assms(1) by (induction \<Gamma> rule: Ctx_Ty_Tm.inducts(1)) (auto simp: assms)
+  using assms(1) by (induction \<Gamma> rule: Ctx_Ty.inducts(1)) (auto simp: assms)
 
 lemma Ty_induct[consumes 1, case_names Var App Unit FunArrow Forall]:
   assumes "\<Gamma> \<turnstile>\<^sub>t\<^sub>y \<tau> : \<kappa>"
@@ -81,21 +80,9 @@ lemma Ty_induct[consumes 1, case_names Var App Unit FunArrow Forall]:
   and FunArrow: "\<And>\<Gamma> \<tau>1 \<tau>2. \<lbrakk> \<Gamma> \<turnstile>\<^sub>t\<^sub>y \<tau>1 : \<star> ; P \<Gamma> \<tau>1 \<star> ; \<Gamma> \<turnstile>\<^sub>t\<^sub>y \<tau>2 : \<star> ; P \<Gamma> \<tau>2 \<star> \<rbrakk> \<Longrightarrow> P \<Gamma> (\<tau>1 \<rightarrow> \<tau>2) \<star>"
   and Forall: "\<And>\<Gamma> a k \<sigma>. \<lbrakk> BTyVar a k # \<Gamma> \<turnstile>\<^sub>t\<^sub>y \<sigma> : \<star> ; P (BTyVar a k # \<Gamma>) \<sigma> \<star> \<rbrakk> \<Longrightarrow> P \<Gamma> (\<forall> a:k. \<sigma>) \<star>"
 shows "P \<Gamma> \<tau> \<kappa>"
-  using assms(1) by (induction \<Gamma> \<tau> \<kappa> rule: Ctx_Ty_Tm.inducts(2)) (auto simp: assms)
+  using assms(1) by (induction \<Gamma> \<tau> \<kappa> rule: Ctx_Ty.inducts(2)) (auto simp: assms)
 
-lemma Tm_induct[consumes 1, case_names Var Abs App TAbs TApp Unit Let]:
-  assumes "\<Gamma> \<turnstile> e : \<tau>"
-  and Var: "\<And>\<Gamma> x \<tau>. \<lbrakk> \<turnstile> \<Gamma> ; BVar x \<tau> \<in> \<Gamma> \<rbrakk> \<Longrightarrow> P \<Gamma> (Var x) \<tau>"
-  and Abs: "\<And>\<Gamma> x \<tau>1 e \<tau>2. \<lbrakk> BVar x \<tau>1 # \<Gamma> \<turnstile> e : \<tau>2 ; P (BVar x \<tau>1 # \<Gamma>) e \<tau>2 \<rbrakk> \<Longrightarrow> P \<Gamma> (\<lambda> x:\<tau>1. e) (\<tau>1 \<rightarrow> \<tau>2)"
-  and App: "\<And>\<Gamma> e1 e2 \<tau>1 \<tau>2. \<lbrakk> \<Gamma> \<turnstile> e1 : (\<tau>1 \<rightarrow> \<tau>2) ; P \<Gamma> e1 (\<tau>1 \<rightarrow> \<tau>2) ; \<Gamma> \<turnstile> e2 : \<tau>1 ; P \<Gamma> e2 \<tau>1 \<rbrakk> \<Longrightarrow> P \<Gamma> (App e1 e2) \<tau>2"
-  and TAbs: "\<And>\<Gamma> a k e \<sigma>. \<lbrakk> BTyVar a k # \<Gamma> \<turnstile> e : \<sigma> ; P (BTyVar a k # \<Gamma>) e \<sigma> \<rbrakk> \<Longrightarrow> P \<Gamma> (\<Lambda> a:k. e) (\<forall> a:k. \<sigma>)"
-  and TApp: "\<And>\<Gamma> a k e \<sigma> \<tau>. \<lbrakk> \<Gamma> \<turnstile> e : (\<forall> a:k. \<sigma>) ; P \<Gamma> e (\<forall> a:k. \<sigma>) ; \<Gamma> \<turnstile>\<^sub>t\<^sub>y \<tau> : k \<rbrakk> \<Longrightarrow> P \<Gamma> (TyApp e \<tau>) \<sigma>[\<tau>/a]"
-  and Unit: "\<And>\<Gamma>. \<turnstile> \<Gamma> \<Longrightarrow> P \<Gamma> Unit TyUnit"
-  and Let: "\<And>\<Gamma> e1 e2 \<tau>1 \<tau>2 x. \<lbrakk> \<Gamma> \<turnstile> e1 : \<tau>1 ; P \<Gamma> e1 \<tau>1 ; BVar x \<tau>1 # \<Gamma> \<turnstile> e2 : \<tau>2 ; P (BVar x \<tau>1 # \<Gamma>) e2 \<tau>2 \<rbrakk> \<Longrightarrow> P \<Gamma> (Let x \<tau>1 e1 e2) \<tau>2"
-shows "P \<Gamma> e \<tau>"
-  using assms(1) by (induction \<Gamma> e \<tau> rule: Ctx_Ty_Tm.inducts(3)) (auto simp: assms)
-
-lemma Ctx_Ty_induct[case_names Ctx_Empty Ctx_TyVar Ctx_Var Ty_Var Ty_App Ty_Unit Ty_FunArrow Ty_Forall]:
+lemma Ctx_Ty_induct_split[case_names Ctx_Empty Ctx_TyVar Ctx_Var Ty_Var Ty_App Ty_Unit Ty_FunArrow Ty_Forall]:
   assumes "P []"
   and "\<And>\<Gamma>' b k2. \<lbrakk> \<turnstile> \<Gamma>' @ \<Gamma> ; P \<Gamma>' ; atom b \<sharp> \<Gamma>' @  \<Gamma> \<rbrakk> \<Longrightarrow> P (BTyVar b k2 # \<Gamma>')"
   and "\<And>\<Gamma>' \<tau> x. \<lbrakk> \<Gamma>' @ \<Gamma> \<turnstile>\<^sub>t\<^sub>y \<tau> : \<star> ; Q \<Gamma>' \<tau> \<star> ; atom x \<sharp> \<Gamma>' @  \<Gamma> \<rbrakk> \<Longrightarrow> P (BVar x \<tau> # \<Gamma>')"
@@ -104,14 +91,15 @@ lemma Ctx_Ty_induct[case_names Ctx_Empty Ctx_TyVar Ctx_Var Ty_Var Ty_App Ty_Unit
   and "\<And>\<Gamma>'. \<lbrakk> \<turnstile> \<Gamma>' @ \<Gamma> ; P \<Gamma>' \<rbrakk> \<Longrightarrow> Q \<Gamma>' TyUnit \<star>"
   and "\<And>\<Gamma>' \<tau>1 \<tau>2. \<lbrakk> \<Gamma>' @ \<Gamma> \<turnstile>\<^sub>t\<^sub>y \<tau>1 : \<star> ; Q \<Gamma>' \<tau>1 \<star> ; \<Gamma>' @  \<Gamma> \<turnstile>\<^sub>t\<^sub>y \<tau>2 : \<star> ; Q \<Gamma>' \<tau>2 \<star> \<rbrakk> \<Longrightarrow> Q \<Gamma>' (\<tau>1 \<rightarrow> \<tau>2) \<star>"
   and "\<And>b k2 \<Gamma>' \<sigma>. \<lbrakk> BTyVar b k2 # \<Gamma>' @ \<Gamma> \<turnstile>\<^sub>t\<^sub>y \<sigma> : \<star> ; Q (BTyVar b k2 # \<Gamma>') \<sigma> \<star> \<rbrakk> \<Longrightarrow> Q \<Gamma>' (\<forall> b : k2 . \<sigma>) \<star>"
-  shows "(\<turnstile> \<Gamma>' @ \<Gamma> \<longrightarrow> P \<Gamma>') \<and> (\<Gamma>' @ \<Gamma> \<turnstile>\<^sub>t\<^sub>y \<tau> : k2 \<longrightarrow> Q \<Gamma>' \<tau> k2)"
+shows "\<turnstile> \<Gamma>' @ \<Gamma> \<longrightarrow> P \<Gamma>'"
+  and "\<Gamma>' @ \<Gamma> \<turnstile>\<^sub>t\<^sub>y \<tau> : k2 \<longrightarrow> Q \<Gamma>' \<tau> k2"
 proof -
   let ?\<Gamma> = "\<Gamma>' @ \<Gamma>"
   let ?P = "\<lambda>x. \<forall>\<Gamma>2. (x = \<Gamma>2 @ \<Gamma>) \<longrightarrow> (P \<Gamma>2)"
   let ?Q = "\<lambda>x y z. \<forall>\<Gamma>2. (x = \<Gamma>2 @ \<Gamma>) \<longrightarrow> (Q \<Gamma>2 y z)"
 
-  have "(\<turnstile> ?\<Gamma> \<longrightarrow> ?P ?\<Gamma>) \<and> (?\<Gamma> \<turnstile>\<^sub>t\<^sub>y \<tau> : k2 \<longrightarrow> ?Q ?\<Gamma> \<tau> k2) \<and> ([] \<turnstile> Unit : TyUnit \<longrightarrow> True)"
-    apply (cases rule: Ctx_Ty_Tm.induct[of "?P" "?Q" "\<lambda>a b c. True"]) apply auto
+  have "(\<turnstile> ?\<Gamma> \<longrightarrow> ?P ?\<Gamma>) \<and> (?\<Gamma> \<turnstile>\<^sub>t\<^sub>y \<tau> : k2 \<longrightarrow> ?Q ?\<Gamma> \<tau> k2)"
+    apply (cases rule: Ctx_Ty.induct[of "?P" "?Q"]) apply auto
   proof (cases)
     fix \<Gamma>2' b \<kappa> \<Gamma>2
     assume a: "\<turnstile> \<Gamma>2'" "\<forall>\<Gamma>2. \<Gamma>2' = \<Gamma>2 @ \<Gamma> \<longrightarrow> P \<Gamma>2" "atom b \<sharp> \<Gamma>2'" "BTyVar b \<kappa> # \<Gamma>2' = \<Gamma>2 @ \<Gamma>"
@@ -131,14 +119,14 @@ proof -
       then show ?thesis using assms(3) a by auto
     qed (simp add: assms(1))
   qed (auto simp: assms(1,4-8))
-  then show ?thesis by simp
+  then show "\<turnstile> \<Gamma>' @ \<Gamma> \<longrightarrow> P \<Gamma>'" and "\<Gamma>' @ \<Gamma> \<turnstile>\<^sub>t\<^sub>y \<tau> : k2 \<longrightarrow> Q \<Gamma>' \<tau> k2" by simp_all
 qed
 
 (* context validity *)
 lemma context_valid_ty: "\<Gamma> \<turnstile>\<^sub>t\<^sub>y \<tau> : \<kappa> \<Longrightarrow> \<turnstile> \<Gamma>"
   by (induction \<Gamma> \<tau> \<kappa> rule: Ty_induct) auto
 lemma context_valid_tm: "\<Gamma> \<turnstile> e : \<tau> \<Longrightarrow> \<turnstile> \<Gamma>"
-  by (induction \<Gamma> e \<tau> rule: Tm_induct) (auto simp: context_valid_ty)
+  by (induction \<Gamma> e \<tau> rule: Tm.induct) (auto simp: context_valid_ty)
 lemmas context_valid = context_valid_ty context_valid_tm
 
 (* \<lbrakk> \<Gamma> \<turnstile> e : t ; atom x \<sharp> \<Gamma> \<rbrakk> \<Longrightarrow> atom x \<sharp> e *)
@@ -149,28 +137,24 @@ proof (induction \<Gamma> \<tau> k rule: Ty_induct)
 qed (auto simp: fresh_Cons)
 
 lemma fresh_in_context_term_var: "\<lbrakk> \<Gamma> \<turnstile> e : \<tau> ; atom (x::var) \<sharp> \<Gamma> \<rbrakk> \<Longrightarrow> atom x \<sharp> e"
-proof (induction \<Gamma> e \<tau> rule: Tm_induct)
-case (Var \<Gamma> x \<tau>)
+proof (induction \<Gamma> e \<tau> rule: Tm.induct)
+case (Tm_Var \<Gamma> x \<tau>)
   then show ?case using fresh_ineq_at_base fresh_not_isin_var by force
 qed (auto simp: fresh_Cons)
 
 lemma fresh_in_context_term_tyvar: "\<lbrakk> \<Gamma> \<turnstile> e : \<tau> ; atom (a::tyvar) \<sharp> \<Gamma> \<rbrakk> \<Longrightarrow> atom a \<sharp> e"
-proof (induction \<Gamma> e \<tau> rule: Tm_induct)
-  case (Abs \<Gamma> x \<tau>1 e \<tau>2)
-  have "atom a \<sharp> \<tau>1" by (metis Abs.hyps Abs.prems Ctx.cases binder.distinct(1) binder.eq_iff(1) context_valid_tm fresh_in_context_ty list.inject list.simps(3))
-  then show ?case by (simp add: Abs fresh_Cons)
+proof (induction \<Gamma> e \<tau> rule: Tm.induct)
+  case (Tm_Abs \<Gamma> x \<tau>1 e \<tau>2)
+  then show ?case using Tm_Abs context_valid_tm fresh_Cons fresh_in_context_ty by fastforce
 next
-  case (Let \<Gamma> e1 e2 \<tau>1 \<tau>2 x)
-  have "atom a \<sharp> \<tau>1" by (metis Ctx.cases Let.hyps(2) Let.prems binder.distinct(1) binder.eq_iff(1) context_valid_tm fresh_in_context_ty list.inject list.simps(3))
-  then show ?case by (simp add: Let fresh_Cons)
+  case (Tm_Let \<Gamma> e1 e2 \<tau>1 \<tau>2 x)
+  then show ?case
+    by (metis (mono_tags, lifting) CtxE(2) binder.fresh(1) context_valid_tm fresh_Cons fresh_in_context_ty fresh_ineq_at_base list.set_intros(1) term.fresh(7))
 qed (auto simp: fresh_Cons fresh_in_context_ty)
 lemmas fresh_in_context = fresh_in_context_ty fresh_in_context_term_var fresh_in_context_term_tyvar
 
 nominal_inductive Ctx avoids
   Ty_Forall: a
-  | Tm_Abs: x
-  | Tm_TAbs: a
-  | Tm_Let: x
 proof (goal_cases)
   case (1 a k \<Gamma> \<sigma>)
   then have "\<turnstile> BTyVar a k # \<Gamma>" by (rule context_valid(1))
@@ -178,15 +162,21 @@ proof (goal_cases)
   obtain c \<sigma>' where 2: "(\<forall> a:k. \<sigma>) = (\<forall> c:k. \<sigma>') \<and> atom a \<sharp> (\<forall> c:k. \<sigma>')" using Abs_fresh_var by auto
   then have "atom a \<sharp> (\<Gamma>, \<forall> c:k. \<sigma>', \<star>)" using 1 fresh_Pair by simp
   then show ?case using 2 fresh_star_def by fastforce
-next
-  case (3 x \<tau>1 \<Gamma> e \<tau>2)
+qed auto
+
+nominal_inductive Tm avoids
+  Tm_Abs: x
+  | Tm_TAbs: a
+  | Tm_Let: x
+proof (goal_cases)
+  case (1 x \<tau>1 \<Gamma> e \<tau>2)
   then have "\<turnstile> BVar x \<tau>1 # \<Gamma>" by (rule context_valid)
   then have 1: "atom x \<sharp> \<Gamma>" by blast
   obtain y e' where 2: "(\<lambda> x:\<tau>1. e) = (\<lambda> y:\<tau>1. e') \<and> atom x \<sharp> (\<lambda> y:\<tau>1. e')" using Abs_fresh_var by auto
   then have "atom x \<sharp> (\<Gamma>, \<lambda> y:\<tau>1. e', \<tau>1 \<rightarrow> \<tau>2)" using 1 fresh_Pair by simp
   then show ?case using 2 fresh_star_def by fastforce
 next
-  case (5 a k \<Gamma> e \<sigma>)
+  case (3 a k \<Gamma> e \<sigma>)
   then have "\<turnstile> BTyVar a k # \<Gamma>" by (rule context_valid)
   then have 1: "atom a \<sharp> \<Gamma>" by blast
   obtain y e' where 2: "(\<Lambda> a:k. e) = (\<Lambda> y:k. e') \<and> atom a \<sharp> (\<Lambda> y:k. e')" using Abs_fresh_var by auto
@@ -194,10 +184,10 @@ next
   then have "atom a \<sharp> (\<Gamma>, \<Lambda> y:k. e', \<forall> y2:k. \<sigma>')" using 1 2 by auto
   then show ?case using 2 3 fresh_star_def by force
 next
-  case (7 \<Gamma> e1 \<tau>1 x e2 \<tau>2)
-  from 7(2) have "\<turnstile> BVar x \<tau>1 # \<Gamma>" by (rule context_valid)
+  case (5 \<Gamma> e1 \<tau>1 x e2 \<tau>2)
+  from 5(2) have "\<turnstile> BVar x \<tau>1 # \<Gamma>" by (rule context_valid)
   then have 1: "atom x \<sharp> \<Gamma>" by blast
-  then have "atom x \<sharp> e1" using "7"(1) fresh_in_context(2) by blast
+  then have "atom x \<sharp> e1" using 5(1) fresh_in_context(2) by blast
   then obtain y e2' where 2: "Let x \<tau>1 e1 e2 = Let y \<tau>1 e1 e2' \<and> atom x \<sharp> Let y \<tau>1 e1 e2'" using Abs_fresh_var by auto
   then have "atom x \<sharp> (\<Gamma>, Let y \<tau>1 e1 e2', \<tau>2)" using 1 fresh_Pair by simp
   then show ?case using 2 fresh_star_def by fastforce
@@ -211,7 +201,7 @@ lemma Ctx_strong_induct[consumes 1, case_names Empty TyVar Var]:
   and TyVar: "\<And>\<Gamma> a k c. \<lbrakk> \<turnstile> \<Gamma> ; (\<And>c. P c \<Gamma>) ; atom a \<sharp> \<Gamma> \<rbrakk> \<Longrightarrow> P c (BTyVar a k # \<Gamma>)"
   and Var: "\<And>\<Gamma> x \<tau> c. \<lbrakk> \<Gamma> \<turnstile>\<^sub>t\<^sub>y \<tau> : \<star> ; atom x \<sharp> \<Gamma> \<rbrakk> \<Longrightarrow> P c (BVar x \<tau> # \<Gamma>)"
 shows "P c \<Gamma>"
-  using assms(1) by (induction \<Gamma> rule: Ctx_Ty_Tm.strong_induct(1)[of _ P "\<lambda>c \<Gamma> \<tau> k. True" "\<lambda>c \<Gamma> e \<tau>. True"]) (auto simp: assms)
+  using assms(1) by (induction \<Gamma> rule: Ctx_Ty.strong_induct(1)[of _ P "\<lambda>c \<Gamma> \<tau> k. True"]) (auto simp: assms)
 
 lemma Ty_strong_induct[consumes 1, case_names Var App Unit FunArrow Forall]:
   fixes c::"'a::fs"
@@ -222,19 +212,6 @@ lemma Ty_strong_induct[consumes 1, case_names Var App Unit FunArrow Forall]:
   and FunArrow: "\<And>\<Gamma> \<tau>1 \<tau>2 c. \<lbrakk> \<Gamma> \<turnstile>\<^sub>t\<^sub>y \<tau>1 : \<star> ; (\<And>c. P c \<Gamma> \<tau>1 \<star>) ; \<Gamma> \<turnstile>\<^sub>t\<^sub>y \<tau>2 : \<star> ; (\<And>c. P c \<Gamma> \<tau>2 \<star>) \<rbrakk> \<Longrightarrow> P c \<Gamma> (\<tau>1 \<rightarrow> \<tau>2) \<star>"
   and Forall: "\<And>a k \<Gamma> \<sigma> c. \<lbrakk> atom a \<sharp> c ; BTyVar a k # \<Gamma> \<turnstile>\<^sub>t\<^sub>y \<sigma> : \<star> ; (\<And>c. P c (BTyVar a k # \<Gamma>) \<sigma> \<star>) \<rbrakk> \<Longrightarrow> P c \<Gamma> (\<forall> a : k . \<sigma>) \<star>"
 shows "P c \<Gamma> \<tau> \<kappa>"
-  using assms(1) by (induction \<Gamma> \<tau> \<kappa> rule: Ctx_Ty_Tm.strong_induct(2)[of _ _ _ "\<lambda>c xs. True" P "\<lambda>c \<Gamma> e \<tau>. True"]) (auto simp: assms fresh_star_def)
-
-lemma Tm_strong_induct[consumes 1, case_names Var Abs App TAbs TApp Unit Let]:
-  fixes c::"'a::fs"
-  assumes "\<Gamma> \<turnstile> e : \<tau>"
-  and Var: "\<And>\<Gamma> x \<tau> c. \<lbrakk> \<turnstile> \<Gamma> ; BVar x \<tau> \<in> \<Gamma> \<rbrakk> \<Longrightarrow> P c \<Gamma> (Var x) \<tau>"
-  and Abs: "\<And>\<Gamma> x \<tau>1 e \<tau>2 c. \<lbrakk> atom x \<sharp> c ; BVar x \<tau>1 # \<Gamma> \<turnstile> e : \<tau>2 ; (\<And>c. P c (BVar x \<tau>1 # \<Gamma>) e \<tau>2) \<rbrakk> \<Longrightarrow> P c \<Gamma> (\<lambda> x:\<tau>1. e) (\<tau>1 \<rightarrow> \<tau>2)"
-  and App: "\<And>\<Gamma> e1 e2 \<tau>1 \<tau>2 c. \<lbrakk> \<Gamma> \<turnstile> e1 : (\<tau>1 \<rightarrow> \<tau>2) ; (\<And>c. P c \<Gamma> e1 (\<tau>1 \<rightarrow> \<tau>2)) ; \<Gamma> \<turnstile> e2 : \<tau>1 ; (\<And>c. P c \<Gamma> e2 \<tau>1) \<rbrakk> \<Longrightarrow> P c \<Gamma> (App e1 e2) \<tau>2"
-  and TAbs: "\<And>\<Gamma> a k e \<sigma> c. \<lbrakk> atom a \<sharp> c ; BTyVar a k # \<Gamma> \<turnstile> e : \<sigma> ; (\<And>c. P c (BTyVar a k # \<Gamma>) e \<sigma>) \<rbrakk> \<Longrightarrow> P c \<Gamma> (\<Lambda> a:k. e) (\<forall> a:k. \<sigma>)"
-  and TApp: "\<And>\<Gamma> a k e \<sigma> \<tau> c. \<lbrakk> \<Gamma> \<turnstile> e : (\<forall> a:k. \<sigma>) ; (\<And>c. P c \<Gamma> e (\<forall> a:k. \<sigma>)) ; \<Gamma> \<turnstile>\<^sub>t\<^sub>y \<tau> : k \<rbrakk> \<Longrightarrow> P c \<Gamma> (TyApp e \<tau>) \<sigma>[\<tau>/a]"
-  and Unit: "\<And>\<Gamma> c. \<turnstile> \<Gamma> \<Longrightarrow> P c \<Gamma> Unit TyUnit"
-  and Let: "\<And>\<Gamma> e1 e2 \<tau>1 \<tau>2 x c. \<lbrakk> atom x \<sharp> c ; \<Gamma> \<turnstile> e1 : \<tau>1 ; (\<And>c. P c \<Gamma> e1 \<tau>1) ; BVar x \<tau>1 # \<Gamma> \<turnstile> e2 : \<tau>2 ; (\<And>c. P c (BVar x \<tau>1 # \<Gamma>) e2 \<tau>2) \<rbrakk> \<Longrightarrow> P c \<Gamma> (Let x \<tau>1 e1 e2) \<tau>2"
-shows "P c \<Gamma> e \<tau>"
-  using assms(1) by (induction \<Gamma> e \<tau> rule: Ctx_Ty_Tm.strong_induct(3)[of _ _ _ "\<lambda>c xs. True" "\<lambda>c \<Gamma> \<tau> k. True" P]) (auto simp: assms fresh_star_def)
+  using assms(1) by (induction \<Gamma> \<tau> \<kappa> rule: Ctx_Ty.strong_induct(2)[of _ _ _ "\<lambda>c xs. True" P]) (auto simp: assms fresh_star_def)
 
 end
