Typing_Lemmas.thy
@@ -5,9 +5,9 @@ begin
 no_notation Set.member  ("(_/ : _)" [51, 51] 50)
 
 lemma fun_ty_lam: "\<lbrakk> \<Gamma> \<turnstile> e : \<tau>1 \<rightarrow> \<tau>2 ; is_value e \<rbrakk> \<Longrightarrow> \<exists>x e'. e = (\<lambda>x:\<tau>1. e')"
-  by (induction \<Gamma> e "\<tau>1 \<rightarrow> \<tau>2" rule: Tm_induct) auto
+  by (induction \<Gamma> e "\<tau>1 \<rightarrow> \<tau>2" rule: Tm.induct) auto
 lemma forall_ty_lam: "\<lbrakk> \<Gamma> \<turnstile> e : (\<forall> a:k. \<sigma>) ; is_value e \<rbrakk> \<Longrightarrow> \<exists>a' e'. e = (\<Lambda> a':k. e')"
-  by (induction \<Gamma> e "(\<forall> a:k. \<sigma>)" rule: Tm_induct) auto
+  by (induction \<Gamma> e "(\<forall> a:k. \<sigma>)" rule: Tm.induct) auto
 
 lemma context_cons_valid[elim]: "\<turnstile> bndr # \<Gamma> \<Longrightarrow> (\<turnstile> \<Gamma> \<Longrightarrow> P) \<Longrightarrow> P"
   by (cases rule: Ctx.cases) (auto simp: context_valid(1))
